src/program_proof/pav/rpc.v
@@ -27,16 +27,16 @@ Lemma wp_NewRpcAuditor ptr_adtr :
   }}}.
 Proof. Admitted.
 
-Lemma wp_CallServPut ptr_cli cli (uid : w64) sl_pk d0 (pk : list w8) :
+Lemma wp_CallServPut ptr_cli addr (uid : w64) sl_pk d0 (pk : list w8) :
   {{{
-    "Hown_cli" ∷ advrpc.Client.own ptr_cli cli ∗
+    "Hown_cli" ∷ advrpc.own_Client ptr_cli addr false ∗
     "Hsl_pk" ∷ own_slice_small sl_pk byteT d0 pk
   }}}
   CallServPut #ptr_cli #uid (slice_val sl_pk)
   {{{
     (err : bool) ptr_dig dig ptr_memb memb ptr_nonmemb nonmemb,
     RET (#ptr_dig, #ptr_memb, #ptr_nonmemb, #err);
-    "Hown_cli" ∷ advrpc.Client.own ptr_cli cli ∗
+    "Hown_cli" ∷ advrpc.own_Client ptr_cli addr false ∗
     "Hsl_pk" ∷ own_slice_small sl_pk byteT d0 pk ∗
     "Herr" ∷ (if err then True else
       "Hown_dig" ∷ SigDig.own ptr_dig dig (DfracOwn 1) ∗
@@ -47,9 +47,9 @@ Proof. Admitted.
 
 (* TODO: this is a direct copy of the Server__Put spec.
 later, need to properly bind these two. *)
-Lemma wp_CallServPut_good ptr_cli cli serv uid nVers sl_pk d0 (pk : list w8) cli_ep :
+Lemma wp_CallServPut_good ptr_cli addr serv uid nVers sl_pk d0 (pk : list w8) cli_ep :
   {{{
-    "Hown_cli" ∷ advrpc.Client.own ptr_cli cli ∗
+    "Hown_cli" ∷ advrpc.own_Client ptr_cli addr true ∗
     "Hvers" ∷ uid ↪[serv.(Server.γvers)] nVers ∗
     "Hsl_pk" ∷ own_slice_small sl_pk byteT d0 pk ∗
     "#Hlb_ep" ∷ mono_nat_lb_own serv.(Server.γepoch) cli_ep
@@ -58,7 +58,7 @@ Lemma wp_CallServPut_good ptr_cli cli serv uid nVers sl_pk d0 (pk : list w8) cli
   {{{
     ptr_sigdig sigdig ptr_lat lat ptr_bound bound err label commit,
     RET (#ptr_sigdig, #ptr_lat, #ptr_bound, #err);
-    "Hown_cli" ∷ advrpc.Client.own ptr_cli cli ∗
+    "Hown_cli" ∷ advrpc.own_Client ptr_cli addr true ∗
     "Hsl_pk" ∷ own_slice_small sl_pk byteT d0 pk ∗
 
     "Hvers" ∷ uid ↪[serv.(Server.γvers)] (word.add nVers (W64 1)) ∗
@@ -80,15 +80,15 @@ Lemma wp_CallServPut_good ptr_cli cli serv uid nVers sl_pk d0 (pk : list w8) cli
   }}}.
 Proof. Admitted.
 
-Lemma wp_CallServGet ptr_cli cli (uid : w64) :
+Lemma wp_CallServGet ptr_cli addr (uid : w64) :
   {{{
-    "Hown_cli" ∷ advrpc.Client.own ptr_cli cli
+    "Hown_cli" ∷ advrpc.own_Client ptr_cli addr false
   }}}
   CallServGet #ptr_cli #uid
   {{{
     (err is_reg : bool) ptr_dig dig sl_hist hist_ref hist ptr_memb memb ptr_nonmemb nonmemb,
     RET (#ptr_dig, slice_val sl_hist, #is_reg, #ptr_memb, #ptr_nonmemb, #err);
-    "Hown_cli" ∷ advrpc.Client.own ptr_cli cli ∗
+    "Hown_cli" ∷ advrpc.own_Client ptr_cli addr false ∗
     "Herr" ∷ (if err then True else
       "#Hown_dig" ∷ SigDig.own ptr_dig dig (DfracOwn 1) ∗
       "Hsl_hist" ∷ own_slice_small sl_hist ptrT (DfracOwn 1) hist_ref ∗
@@ -98,55 +98,55 @@ Lemma wp_CallServGet ptr_cli cli (uid : w64) :
   }}}.
 Proof. Admitted.
 
-Lemma wp_CallServSelfMon ptr_cli cli (uid : w64) :
+Lemma wp_CallServSelfMon ptr_cli addr (uid : w64) :
   {{{
-    "Hown_cli" ∷ advrpc.Client.own ptr_cli cli
+    "Hown_cli" ∷ advrpc.own_Client ptr_cli addr false
   }}}
   CallServSelfMon #ptr_cli #uid
   {{{
     (err : bool) ptr_dig dig ptr_nonmemb nonmemb, RET (#ptr_dig, #ptr_nonmemb, #err);
-    "Hown_cli" ∷ advrpc.Client.own ptr_cli cli ∗
+    "Hown_cli" ∷ advrpc.own_Client ptr_cli addr false ∗
     "Herr" ∷ (if err then True else
       "#Hown_dig" ∷ SigDig.own ptr_dig dig (DfracOwn 1) ∗
       "Hown_nonmemb" ∷ NonMemb.own ptr_nonmemb nonmemb (DfracOwn 1))
   }}}.
 Proof. Admitted.
 
-Lemma wp_CallServAudit ptr_cli cli (ep : w64) :
+Lemma wp_CallServAudit ptr_cli addr (ep : w64) :
   {{{
-    "Hown_cli" ∷ advrpc.Client.own ptr_cli cli
+    "Hown_cli" ∷ advrpc.own_Client ptr_cli addr false
   }}}
   CallServAudit #ptr_cli #ep
   {{{
     (err : bool) ptr_upd upd, RET (#ptr_upd, #err);
-    "Hown_cli" ∷ advrpc.Client.own ptr_cli cli ∗
+    "Hown_cli" ∷ advrpc.own_Client ptr_cli addr false ∗
     if negb err then
       "Hown_upd" ∷ UpdateProof.own ptr_upd upd (DfracOwn 1)
     else True
   }}}.
 Proof. Admitted.
 
-Lemma wp_CallAdtrUpdate ptr_cli cli ptr_upd upd d0 :
+Lemma wp_CallAdtrUpdate ptr_cli addr ptr_upd upd d0 :
   {{{
-    "Hown_cli" ∷ advrpc.Client.own ptr_cli cli ∗
+    "Hown_cli" ∷ advrpc.own_Client ptr_cli addr false ∗
     "Hown_upd" ∷ UpdateProof.own ptr_upd upd d0
   }}}
   CallAdtrUpdate #ptr_cli #ptr_upd
   {{{
     (err : bool), RET #err;
-    "Hown_cli" ∷ advrpc.Client.own ptr_cli cli ∗
+    "Hown_cli" ∷ advrpc.own_Client ptr_cli addr false ∗
     "Hown_upd" ∷ UpdateProof.own ptr_upd upd d0
   }}}.
 Proof. Admitted.
 
-Lemma wp_CallAdtrGet ptr_cli cli (ep : w64) :
+Lemma wp_CallAdtrGet ptr_cli addr (ep : w64) :
   {{{
-    "Hown_cli" ∷ advrpc.Client.own ptr_cli cli
+    "Hown_cli" ∷ advrpc.own_Client ptr_cli addr false
   }}}
   CallAdtrGet #ptr_cli #ep
   {{{
     (err : bool) ptr_adtrInfo adtrInfo, RET (#ptr_adtrInfo, #err);
-    "Hown_cli" ∷ advrpc.Client.own ptr_cli cli ∗
+    "Hown_cli" ∷ advrpc.own_Client ptr_cli addr false ∗
     if negb err then
       "Hown_info" ∷ AdtrEpochInfo.own ptr_adtrInfo adtrInfo (DfracOwn 1)
     else True
